proofs/Axioms.lean
@@ -21,3 +21,4 @@ import Statements
 #print axioms Protocol.Statements.check_S13_valid_id
 #print axioms Protocol.Statements.check_S3_S4_parse
 #print axioms Protocol.Statements.check_C3_serialize
+#print axioms Protocol.Statements.check_C3_parse
